Source/DafnyStandardLibraries/examples/FileIO/ReadFromFile.dfy
@@ -1,0 +1,32 @@
+/*******************************************************************************
+ *  Copyright by the contributors to the Dafny Project
+ *  SPDX-License-Identifier: MIT
+ *******************************************************************************/
+
+module ReadFromFile {
+  import Std.FileIO
+
+  @Test
+  method Test() {
+    // TODO: extern function for the expected error prefix
+    theMain("examples/FileIO/../FileIO/data.txt", "");
+  }
+
+  method theMain(dataPath: string, expectedErrorPrefix: string) {
+
+      // Happy path: read from the data file, and check that we see the expected content.
+    {
+      var expectedStr := "Hello world\nGoodbye\n";
+      var res := FileIO.ReadFile(dataPath);
+      expect res.Success?, "unexpected failure: " + res.error;
+      expect res.value == expectedStr;
+    }
+
+      // Failure path: attempting to read from a blank file path should never work.
+    {
+      var res := FileIO.ReadFile("");
+      expect res.Failure?, "unexpected success";
+      expect expectedErrorPrefix <= res.error, "unexpected error message: " + res.error;
+    }
+  }
+}
